---
title: Lezione 17 (2024-10-17)
---

## Derivate elementari

- $$(x^{n})' = n x^{n - 1}, \ n \in \N$$

  <details>
  <summary>Dimostrazione</summary>

  $$
  \begin{darray}{l}
  \lim_{h \to 0} \frac{(x + h)^{n} - x^{n}}{h} = \\
  \lim_{h \to 0} \frac{\sum_{k = 0}^{n} \binom{n}{k} x^{k} h^{n - k} - x^{n}}{h} \\
  \lim_{h \to 0} \frac{\sum_{k = 0}^{n - 2} \binom{n}{k} x^{k} h^{n - k} + n x^{n - 1} + x^{n} - x^{n}}{h} \\
  \lim_{h \to 0} \frac{h \PR{\sum_{k = 0}^{n - 2} \binom{n}{k} x^{k} h^{n - k - 1} n x^{n - 1}}}{h} \\
  \lim_{h \to 0} \sum_{k = 0}{n - 2} \binom{n}{k} x^{k} n^{n - k - 1} + n x^{n - 1} = n x^{n - 1}
  \end{darray}
  $$

  </details>

- $$(x^{-1})' = - \frac{1}{x^{2}}$$

  <details>
  <summary>Dimostrazione</summary>

  $$
  \begin{darray}{l}
  \lim_{h \to 0} \frac{(x + h)^{-1} - x^{-1}}{h} = \\
  \lim_{h \to 0} \frac{\frac{1}{x + h} - \frac{1}{x}}{h} = \\
  \lim_{h \to 0} \frac{\frac{x - h - x}{x (x + h)}}{h} = \\
  \lim_{h \to 0} \frac{-1}{x (x + h)} = - \frac{1}{x^{2}}
  \end{darray}
  $$

  </details>

- $$(e^{x})' = e^{x}$$

  <details>
  <summary>Dimostrazione</summary>

  $$
  \begin{darray}{l}
  \lim_{h \to 0} \frac{e^{x + h} - e^{x}}{h} = \\
  \lim_{h \to 0} \frac{e^{x} (e^{h} - 1)}{h} = \\
  \lim_{h \to 0} e^{x} \frac{e^{h} - e^{x}}{h} = e^{x}
  \end{darray}
  $$

  </details>
