---
title: Lezione 18 (2024-10-21)
---

## Derivate elementari

- $$\dx{\ln{x}} = \frac{1}{x}$$

  <details>
  <summary>Dimostrazione</summary>

  $$
  \begin{darray}{l}
  \lim_{h \to 0} \frac{\ln{h + x} - \ln{x}}{h} =                        \\
  \lim_{h \to 0} \frac{\ln{\frac{x + h}{x}}}{h} =                       \\
  \lim_{h \to 0} \frac{\ln{1 + \frac{h}{x}}}{\frac{h}{x}} \frac{1}{x} = \\
  \lim_{h \to 0} 1 \frac{1}{x} = \frac{1}{x}
  \end{darray}
  $$

  </details>

- $$\dx{\sin{x}} = \cos{x}$$

  <details>
  <summary>Dimostrazione</summary>

  $$
  \begin{darray}{l}
  \lim_{h \to 0} \frac{\sin{x + h} - \sin{x}}{h} =                                      \\
  \lim_{h \to 0} \frac{\sin{x} \cos{h} + \sin{h} \cos{x} - \sin{x}}{h} =                \\
  \lim_{h \to 0} \frac{\sin{x} \PR{\cos{h} + \frac{\sin{h} \cos{x}}{\sin{x}} - 1}}{h} = \\
  \lim_{h \to 0} \sin{x} \frac{\cos{h} - 1}{h} + \frac{\sin{h} \cos{x}}{h} =            \\
  \lim_{h \to 0} \sin{x} \frac{\cos{h} - 1}{h^{2}} h +\cos{x} =                         \\
  \lim_{h \to 0} -\sin{x} \frac{1}{2} h +\cos{x} = \cos{x}
  \end{darray}
  $$

  </details>

- $$\dx{\cos{x}} = -\sin{x}$$

  <details>
  <summary>Dimostrazione</summary>

  $$
  \begin{darray}{l}
  \lim_{h \to 0} \frac{\cos{x + h} - \cos{x}}{h} =                                      \\
  \lim_{h \to 0} \frac{\cos{x} \cos{h} - \sin{x} \sin{h} - \cos{x}}{h} =                \\
  \lim_{h \to 0} \frac{\cos{x} \PR{\cos{h} - \frac{\sin{x} \sin{h}}{\cos{x}} - 1}}{h} = \\
  \lim_{h \to 0} \cos{x} \frac{\cos{h} - 1}{h} - \frac{\sin{x} \sin{h}}{h} =            \\
  \lim_{h \to 0} \cos{x} \frac{\cos{h} - 1}{h^{2}} h - \sin{x} =                        \\
  \lim_{h \to 0} - \cos{x} \frac{1}{2} h - \sin{x} = -\sin{x}
  \end{darray}
  $$

  </details>

## Regole di derivazione

### Linearit√†

Date $$f(x)$$, $$g(x)$$ derivabili in $$x_{0}$$:

$$
\dx{a f(x_{0}) + b g(x_{0})} = a \dx{f(x_{0})} + b \dx{g(x_{0})}
$$

### Regola di Leibniz

Date $$f(x)$$, $$g(x)$$ derivabili in $$x_{0}$$:

$$
\dx{f(x_{0}) g(x_{0})} = f(x_{0}) \dx{g(x_{0})} + g({x_0}) \dx{f(x_{0})}
$$

### Regola della catena

Date $$g(x)$$ derivabile in $$x_{0}$$ e $$f(x)$$ derivabile in
$$y_{0} = g(x_{0})$$:

$$
\dx{\PR{f \circ g}(x_{0})} = \dx{f(g(x_{0}))} \dx{g(x_{0})}
$$
